src/linear/adt/Stack.dfy
@@ -100,10 +100,225 @@ class Stack1 extends Stack {
   {
     x := list.Pop();
   }
+
+  // method Reverse()
+  //   modifies this, Repr()
+  //   requires Valid()
+  //   ensures Valid()
+  //   ensures Model() == Seq.Rev(old(Model()))
+  //   ensures Repr() == old(Repr())
 }
 
+function method abs(x: int): int
+{
+  if x < 0 then
+    -x
+  else
+    x
+}
+
+// lemma lemma1(v: array<int>, i: int)
+//   requires forall i | 0 <= i < v.Length - 1 :: abs(v[i]) <= abs(v[i+1])
+//   requires 0 <= i <= v.Length
+//   ensures forall j | 0 <= j < i :: abs(v[j]) <= abs(v[i])
+
+method Reverse(st: Stack)
+  modifies st, st.Repr()
+  requires st.Valid()
+  ensures st.Valid()
+  ensures st.Model() == Seq.Rev(old(st.Model()))
+  ensures forall x | x in st.Repr() - old(st.Repr()) :: fresh(x)
+
+method split(v: array<int>, neg: Stack, pos: Stack)
+  modifies pos, pos.Repr(), neg, neg.Repr()
+  requires neg.Valid()
+  requires neg.Empty()
+  requires pos.Valid()
+  requires pos.Empty()
+  requires pos.Repr() !! neg.Repr()
+
+  ensures pos.Valid()
+  ensures neg.Valid()
+  ensures pos.Repr() !! neg.Repr()
+
+  ensures forall x | x in neg.Repr() - old(neg.Repr()) :: fresh(x)
+  ensures forall x | x in neg.Model() :: x < 0
+  ensures forall i | 0 <= i < |neg.Model()| - 1 :: abs(neg.Model()[i]) >= abs(neg.Model()[i+1])
+
+  ensures forall x | x in pos.Repr() - old(pos.Repr()) :: fresh(x)
+  ensures forall x | x in pos.Model() :: x >= 0
+  ensures forall i | 0 <= i < |pos.Model()| - 1 :: abs(pos.Model()[i]) >= abs(pos.Model()[i+1])
+
+  ensures Seq.MElems(neg.Model()) + Seq.MElems(pos.Model()) == Seq.MElems(v[..])
+/*
+{
+  var i := 0;
+  while i < v.Length
+    invariant i <= v.Length
+
+    invariant forall i | 0 <= i < v.Length - 1 :: abs(v[i]) <= abs(v[i+1])
+
+    invariant neg.Repr() !! pos.Repr()
+    invariant forall x | x in neg.Repr() :: fresh(x)
+    invariant forall x | x in pos.Repr() :: fresh(x)
+    // invariant neg != pos
+
+    invariant forall x | x in neg.Repr() :: fresh(x)
+    invariant neg.Valid()
+    invariant forall x | x in neg.Model() :: x < 0
+    invariant forall i | 0 <= i < |neg.Model()| - 1 :: abs(neg.Model()[i]) >= abs(neg.Model()[i+1])
+    // invariant forall i | 0 <= i < |neg.Model()| - 1 :: neg.Model()[i] <= neg.Model()[i+1]
+
+    invariant forall x | x in pos.Repr() :: fresh(x)
+    invariant pos.Valid()
+    invariant forall x | x in pos.Model() :: x >= 0
+    invariant forall i | 0 <= i < |pos.Model()| - 1 :: abs(pos.Model()[i]) >= abs(pos.Model()[i+1])
+    // invariant forall i | 0 <= i < |neg.Model()| - 1 :: neg.Model()[i] >= neg.Model()[i+1]
+
+    invariant Seq.MElems(neg.Model()) + Seq.MElems(pos.Model())
+      == Seq.MElems(v[..i])
+
+  {
+    lemma1(v, i);
+    assert forall j | 0 <= j < i :: abs(v[j]) <= abs(v[i]);
+    if v[i] < 0 {
+      assert Seq.MElems(neg.Model()) + Seq.MElems(pos.Model())
+        == Seq.MElems(v[..i]);
+      assert Seq.MElems(neg.Model())
+        == Seq.MElems(v[..i]) - Seq.MElems(pos.Model());
+      assert forall x | x in Seq.MElems(neg.Model()) :: x in Seq.MElems(v[..i]) - Seq.MElems(pos.Model());
+      assert forall x | x in Seq.MElems(neg.Model()) :: x in Seq.MElems(v[..i]);
+      // assert forall x | x in Seq.MElems(neg.Model()) :: x in neg.Model();
+      assert forall x | x in neg.Model() :: x in Seq.MElems(neg.Model());
+      assert forall x | x in neg.Model() :: x in v[..i];
+      assert forall x | x in neg.Model() :: exists j | 0 <= j < i :: v[j] == x;
+      assert forall x | x in neg.Model() :: abs(v[i]) >= x;
+      assert |neg.Model()| > 0 ==> neg.Model()[0] in neg.Model();
+      assert |neg.Model()| > 0 ==> abs(v[i]) >= neg.Model()[0];
+      // assert forall j | 0 <= j < |neg.Model()| :: neg.Model()[j] in v[..i];
+      // assert forall j | 0 <= j < |neg.Model()| :: abs(neg.Model()[j]) <= abs(v[i]);
+      // assert forall j | 0 <= j < |neg.Model()| :: neg.Model()[j] <= v[i];
+      neg.Push(v[i]);
+    } else {
+      assert Seq.MElems(pos.Model()) + Seq.MElems(neg.Model())
+        == Seq.MElems(v[..i]);
+      assert Seq.MElems(pos.Model())
+        == Seq.MElems(v[..i]) - Seq.MElems(neg.Model());
+      assert forall x | x in Seq.MElems(pos.Model()) :: x in Seq.MElems(v[..i]) - Seq.MElems(neg.Model());
+      assert forall x | x in Seq.MElems(pos.Model()) :: x in Seq.MElems(v[..i]);
+      // assert forall x | x in Seq.MElems(pos.Model()) :: x in pos.Model();
+      assert forall x | x in pos.Model() :: x in Seq.MElems(pos.Model());
+      assert forall x | x in pos.Model() :: x in v[..i];
+      assert forall x | x in pos.Model() :: exists j | 0 <= j < i :: v[j] == x;
+      assert forall x | x in pos.Model() :: abs(v[i]) >= x;
+      assert |pos.Model()| > 0 ==> pos.Model()[0] in pos.Model();
+      assert |pos.Model()| > 0 ==> abs(v[i]) >= pos.Model()[0];
+      assert forall x | x in pos.Model() :: exists j | 0 <= j < i :: v[j] == x;
+      assert forall x | x in pos.Model() :: abs(v[i]) >= x;
+      assert |pos.Model()| > 0 ==> pos.Model()[0] in pos.Model();
+      assert |pos.Model()| > 0 ==> abs(v[i]) >= pos.Model()[0];
+      pos.Push(v[i]);
+    }
+    i := i + 1;
+  }
+}
+*/
+
+method FillFromStack(r: array<int>, i: nat, st: Stack) returns (l: nat)
+  modifies st, st.Repr()
+  requires st.Valid()
+  requires i + |st.Model()| <= r.Length
+  ensures st.Valid()
+  ensures st.Empty()
+  ensures forall x | x in st.Repr() - old(st.Repr()) :: fresh(x)
+  ensures r[i..i+old(|st.Model()|)] == old(st.Model())
+  ensures Seq.MElems(r[i..i+old(|st.Model()|)]) == Seq.MElems(old(st.Model()))
+  ensures l == i + old(|st.Model()|)
+
+method reordenandoLaCola(v: array<int>) returns (r: array<int>)
+  requires forall i | 0 <= i < v.Length - 1 :: abs(v[i]) <= abs(v[i+1])
+  ensures v.Length == r.Length
+  ensures Array.melems(v) == Array.melems(r)
+  ensures forall i | 0 <= i < r.Length - 1 :: r[i] <= r[i+1]
+{
+  var neg: Stack := new Stack1();
+  var pos: Stack := new Stack1();
+  split(v, neg, pos);
+  assert Seq.MElems(neg.Model()) + Seq.MElems(pos.Model()) == Seq.MElems(v[..]);
+  calc == {
+    |neg.Model()| + |pos.Model()|;
+    |Seq.MElems(neg.Model())| + |Seq.MElems(pos.Model())|;
+    |Seq.MElems(neg.Model()) + Seq.MElems(pos.Model())|;
+    |Seq.MElems(v[..])|;
+    |v[..]|;
+    v.Length;
+  }
+  assert |neg.Model()| + |pos.Model()| == |v[..]| == v.Length;
+  var i := 0;
+  r := new int[v.Length];
+  ghost var onegmodel := neg.Model();
+  ghost var oposmodel := pos.Model();
+  assert |onegmodel| + |oposmodel| == v.Length;
+  assert neg.Repr() !! pos.Repr();
+  assert pos !in neg.Repr();
+  assert pos != neg;
+  i := FillFromStack(r, i, neg);
+  assert |onegmodel| + |oposmodel| == v.Length;
+  assert i == |onegmodel|;
+  assert pos.Valid();
+  Reverse(pos);
+  assert pos.Model() == Seq.Rev(oposmodel);
+  assert |pos.Model()| == |oposmodel|;
+  assert i + |pos.Model()| == i + |oposmodel| == |onegmodel| + |oposmodel| == v.Length == r.Length;
+  i := FillFromStack(r, i, pos);
+  /*
+  while !neg.Empty()
+    decreases neg.Model()
+
+    invariant 0 <= i <= r.Length
+
+    invariant neg.Valid()
+    invariant pos.Valid()
+    invariant forall x | x in neg.Repr() :: fresh(x)
+    invariant forall x | x in pos.Repr() :: fresh(x)
+
+    invariant r[..i] + neg.Model() == onegmodel
+    invariant forall j | 0 <= j < i-1 :: r[j] <= r[j+1]
+  {
+    var x := neg.Pop();
+    r[i] := x;
+    i := i + 1;
+  }
+
+  Reverse(pos);
+  // pos.Reverse();
+  ghost var oposmodel := pos.Model();
+  assert r[..i] == onegmodel;
+  assert pos.Model() == oposmodel;
+  while !pos.Empty()
+    decreases pos.Model()
+
+    invariant 0 <= i <= r.Length
+
+    invariant neg.Valid()
+    invariant pos.Valid()
+    invariant forall x | x in neg.Repr() :: fresh(x)
+    invariant forall x | x in pos.Repr() :: fresh(x)
+
+    invariant r[..i] + pos.Model() == onegmodel + oposmodel
+    invariant forall j | 0 <= j < i-1 :: r[j] <= r[j+1]
+  {
+    var x := pos.Pop();
+    r[i] := x;
+    i := i + 1;
+  }
+  assert i == r.Length;
+     */
+}
+
+/*
 method EvalPostfix(s: string) returns (res: int)
-  requires forall c | c in s :: c in "0123456789+-*/"
+  requires forall c | c in s :: c in "0123456789+-*//*"
 {
   var st: Stack := new Stack1();
   var i := 0;
@@ -203,7 +418,9 @@ method Print(st: Stack)
 
 method Main() {
   var st: Stack := new Stack1();
-  st.Push(1);
+  st.Push(3);
   st.Push(2);
+  st.Push(1);
   Print(st);
 }
+*/
